hello

examples/auction/Auction.v
@@ -6,7 +6,10 @@ From ConCert.Execution Require Import Blockchain.
 From ConCert.Execution Require Import Monad.
 From ConCert.Execution Require Import ResultMonad.
 From ConCert.Execution Require Import Serializable.
+From ConCert.Execution Require Import ContractCommon.
 From ConCert.Utils Require Import RecordUpdate.
+From ConCert.Utils Require Import Automation.
+From ConCert.Utils Require Import Extras.
 
 Section Auction.
   Context `{Base : ChainBase}.
@@ -15,7 +18,7 @@ Section Auction.
   
   Inductive AuctionState :=
   | not_sold_yet : AuctionState
-  | sold : AuctionState.
+  | sold : Address -> AuctionState.
 
   (** 
       /// Type of the parameter to the `init` function
@@ -46,7 +49,7 @@ Section Auction.
         minimum_raise : Amount;
         current_price : Amount;
         highest_bidder : option Address;
-        last_action: nat;
+        creation_slot : nat;
       }.
 
   Definition Error : Type := nat.
@@ -106,6 +109,8 @@ Section Auction.
           None          (* Initial highest bidder *)
           (current_slot chain) (* Slot of contract initialization *)
       ).
+
+  Print act_transfer.
   
   (* TODO: Do we need next_state? *)
   Definition receive
@@ -115,23 +120,158 @@ Section Auction.
     (msg : option Msg)
     : result (State * list ActionBody) Error :=
     match msg with
+    (* Placing a bid. *)
     | Some bid =>
         let price := current_price state in
         let min_raise := minimum_raise state in
         let bid_amount := ctx_amount ctx in
+        let curr_slot := current_slot chain in
+        let start_slot := creation_slot state in
+        let dur := duration state in
+        let bidder := ctx_from ctx in
+        (* Ensure bidder is not a contract *)
+        do if address_is_contract bidder
+           then Err default_error
+           else Ok tt;
+        (* Ensure auction has not ended *)
+        do if (start_slot + dur <=? curr_slot)%nat
+           then Ok tt
+           else Err default_error;
+        (* Ensure auction is still active. *)
+        do match auction_state state with
+           | not_sold_yet => Ok tt
+           | _ => Err default_error
+           end;
         (* Ensure new bid raises by at least the minimum raise amount. *)
         do if bid_amount <? price + min_raise
            then Err default_error
            else Ok tt;
-        (* TODO: Update new highest bidder and return money! *)
-        Ok (state, [])
+        (* If there was a previous highest bidder, return the bid. *)
+        let action_list :=
+          match highest_bidder state with
+          | None => []
+          | Some addr => [act_transfer addr price]
+          end in
+        (* Update the state with the new highest bid and bidder *)
+        let new_state :=
+          state<| current_price := bid_amount |>
+               <| highest_bidder := Some bidder |>
+        in
+        Ok (new_state, action_list)
     | Some view => Ok (state, [])
     | Some view_highest_bid => Ok (state, [])
-    | Some finalize => Ok (state, [])
+    | Some finalize =>
+        let curr_slot := current_slot chain in
+        let start_slot := creation_slot state in
+        let dur := duration state in
+        (* Ensure the auction has ended *)
+        do if (curr_slot <? start_slot + dur)%nat
+           then Ok tt
+           else Err default_error;
+        (* Ensure the auction has not been finalized *)
+        do match auction_state state with
+           | not_sold_yet => Ok tt
+           | _ => Err default_error
+           end;
+        (* TODO: How to deal with unsold item? *)
+        do bidder <- result_of_option (highest_bidder state) default_error;
+        let new_state := state<| auction_state := sold bidder |> in
+        Ok (new_state, [act_transfer (seller state) (current_price state)])
     | None => Err default_error
     end.
-
+  
   Definition contract : Contract Setup Msg State Error :=
     build_contract init receive.
 
 End Auction.
+Section Theories.
+  Context `{Base : ChainBase}.
+  Open Scope Z.
+  Definition bidder ctx new_state :=
+    let caddr := ctx_contract_address ctx in
+    match highest_bidder new_state with
+    | Some addr => (caddr =? addr)%address = false
+    | None => False
+    end.
+  (*
+  Lemma try_bidder : forall prev_state new_state chain ctx new_acts,
+      (address_is_contract (ctx_contract_address ctx) = true) -> 
+      receive chain ctx prev_state (Some bid) = Ok (new_state, new_acts) ->
+      bidder ctx new_state.
+  Proof.
+    intros.
+    unfold bidder.
+    destruct new_state; cbn.
+    destruct highest_bidder0 eqn:Hb.
+    - cbn in *.
+      remember (address_is_contract (ctx_from ctx)).
+      destruct b; try congruence.
+      cbn in *
+      do 2 (cbn in *; destruct_match in H; try congruence).
+      destruct ctx; cbn in *; vm_compute in H; try congruence.
+      inversion H.
+      rewrite <- H7.
+      subst.
+      inversion_clear H.
+    - do 5 (cbn in *; destruct_match in H; try congruence);
+      destruct ctx; cbn in *;
+      vm_compute in H;
+      try congruence. *)
+  
+  Lemma no_self_calls bstate caddr:
+    reachable bstate ->
+    env_contracts bstate caddr = Some (Auction.contract : WeakContract) ->
+    Forall (fun abody => match abody with
+                      | act_transfer to _ => (to =? caddr)%address = false
+                      | _ => False
+                      end) (outgoing_acts bstate caddr).
+  Proof.
+(*    intros.
+    eapply deployed_contract_state_typed in H0 as H'; auto.
+    destruct H' as [cstate H'].
+    generalize dependent H0.
+    generalize dependent H.*)
+    contract_induction; intros; cbn in *; auto.
+    - now inversion IH.
+    - apply Forall_app. split; last apply IH.
+      clear IH.
+      unfold receive in receive_some.
+      destruct_match in receive_some; try inversion receive_some.
+      cbn in *; destruct_match in receive_some; try congruence.
+      + remember (address_is_contract (ctx_from ctx)).
+        destruct b; try congruence.
+        do 4 (destruct_match in receive_some; cbn in *; try congruence).
+        inversion_clear H0.
+        * destruct new_state.
+    - apply IH.
+    - split.
+      + 
+
+      apply Forall_nil.
+    - inversion IH.
+      apply H2.
+    - apply Forall_app.
+      split; try apply IH.
+      unfold receive in receive_some.
+      destruct_match as [[]|] in receive_some.
+      + destruct prev_state.
+        do 4 (destruct_match in receive_some; cbn in *; try congruence).
+        destruct_match in receive_some; cbn in *.
+       
+        * inversion_clear receive_some.
+          constructor; auto.
+          eapply address_eq_ne; auto.
+          intro; subst.
+          
+          admit. (* Highest bidder should not be able to be a contract *)
+        * now inversion receive_some.
+      + inversion receive_some; auto.
+      + inversion receive_some; auto.
+      + do 3 (destruct_match in receive_some; cbn in *; try congruence).
+        inversion_clear receive_some.
+        constructor; try constructor.
+        admit. (* Similar to previous admit. *)
+      + congruence.
+    - apply Forall_app; split; [| now inversion IH].
+   *) 
+                
